---
title: "hw03"
author: "Victor Huang"
date: "1/27/2022"
output: pdf_document
---

```{r setup, include=FALSE}
knitr::opts_chunk$set(echo = TRUE)
library(ggplot2)
library(tidyverse)
library(plotrix)
library(mosaic)
```

## Q1. (Exercise 6.4)
$f(x;\theta) = \frac{x^{3}e^{\frac{-x}{\theta}}}{6 \theta ^{4}}$ for $x \geq 0$, find maximum likelihood estimate of $\theta$
$$L(\theta) = \Pi^{n}_{i = 1}f(x; \theta)$$
$$L(\theta) = \Pi^{n}_{i = 1}\frac{x^{3}e^{\frac{-x}{\theta}}}{6 \theta ^{4}}$$
$$L(\theta) = \frac{(\Pi x)^3e^{\frac{-  \sum x_{i}}{\theta}}}{6^n \theta^{4n}}$$
We can log both sides and set derivative equal to 0 to get MLE
$$log(L(\theta)) = 3log(\Pi x_{i}) - \frac{\sum x_{i}}{\theta} - nlog(6) - 4nlog(\theta)$$
$$\frac{d}{d \theta} log(L(\theta)) = 0$$
$$0 + \frac{\sum^{n}_{i = 1}x_{i}}{\theta ^2} - 0 - \frac{4n}{\theta} = 0$$
$$\frac{\sum^{n}_{i = 1}x_{i}}{\theta ^2} = \frac{4n}{\theta}$$
$$\frac{\sum^{n}_{i = 1}x_{i}}{\theta} = 4n$$
$$\sum^{n}_{i = 1}x_{i} = 4n \theta$$
$$\hat \theta = \frac{1}{4n} \sum^{n}_{i = 1}x_{i}$$
$$\hat \theta = \frac{1}{4n} \bar x$$
check
$$l''(\theta) = -2\frac{(4n)^3}{(\sum^{n}_{i=1}x_{i})^2} + \frac{(4n)^3}{(\sum^{n}_{i=1}x_{i})^2} = -\frac{(4n)^3}{(\sum^{n}_{i=1}x_{i})^2} < 0$$

## Q2. (Exercise 6.6)
a). $f(x; \theta) = e^{\theta - x}$ for $x > \theta > 0$. Find the MLE of $\theta$
$$L(\theta) = \Pi^{n}_{i = 1}f(x; \theta)$$
$$L(\theta) = \Pi^{n}_{i = 1}e^{\theta - x}$$
$$L(\theta) = \Pi^{n}_{i = 1}e^{-(x - \theta)}$$
$$L(\theta) = e^{- \sum^{n}_{i=1}(x_{i} - \theta)}$$
$$L(\theta) = e^{- \sum^{n}_{i=1}x_{i}}e^{n \theta}$$
$$log(L(\theta)) = -nlog(e^{n \theta})$$
$$L(\theta) = \theta n - \sum^{n}_{i=1}x_{i}$$
$$L'(\theta) = n - 0 = n$$
$$n \neq 0$$
Therefore, MLE is not possible

b). MLE is still not possible and does not exist. 


## Q3. (Exercise 6.12)

$$X_{1},X_{2} = N(\mu, 3^2)$$
$$Y_{1},Y_{2} = N(2 \mu, 3^2)$$
$$f(x) = \frac{1}{\sigma \sqrt{2 \pi}}e^{\frac{1}{2}(\frac{x - \mu}{\sigma})^2}$$
$$L(p) = P(X_1 = 3, X_2 = -1, Y_1 = 3, Y_2 = 2) = P(X_1 = 3)P(X_2 = -1)P(Y_1 = 3)P(Y_2 = 2)$$
$$L(p) = \frac{1}{3 \sqrt{2 \pi}}e^{\frac{-1}{2}(\frac{3 - \mu}{\sigma})^2}. \frac{1}{3 \sqrt{2 \pi}}e^{\frac{-1}{2}(\frac{-1 - \mu}{\sigma})^2}. \frac{1}{3 \sqrt{2 \pi}}e^{\frac{-1}{2}(\frac{3 - 2\mu}{\sigma})^2}. \frac{1}{3 \sqrt{2 \pi}}e^{\frac{-1}{2}(\frac{3 - 2\mu}{\sigma})^2}$$
$$L(p) = (\frac{1}{3 \sqrt{2 \pi}})^4e^{\frac{-1}{2}(\frac{3 - \mu}{\sigma})^2 + \frac{-1}{2}(\frac{-1 - \mu}{\sigma})^2 + \frac{-1}{2}(\frac{3 - 2\mu}{\sigma})^2 + \frac{-1}{2}(\frac{3 - 2\mu}{\sigma})^2}$$
$$l(p) = log(\frac{1}{324 \pi^2}) + \frac{-1}{2}((\frac{3 - \mu}{3})^2 + (\frac{-1 - \mu}{3})^2 + (\frac{3 - 2\mu}{3})^2 + (\frac{2 - 2\mu}{3})^2)$$
$$l(p) = log(\frac{1}{324 \pi^2}) - \frac{1}{18}(23 - 24 \mu + 10 \mu^2)$$
$$l'(p) = \frac{1}{18}(20 \mu - 24) = \frac{-1}{18}(20 \mu -24)$$
$$\frac{-1}{18}(20 \mu -24) = 0$$
$$\mu = \frac{6}{5}$$
check
$$l'(p) = \frac{-20}{18} \mu + \frac{24}{18}$$
$$l''(p) = \frac{-20}{18} < 0$$

